Manual/Terms.lean
@@ -232,7 +232,7 @@ open D
 ## Leading `.`
 
 When an identifier begins with a dot (`.`), the type that the elaborator expects for the expression is used to resolve it, rather than the current namespace and set of open namespaces.
-{tech}[Generalized field notation] is related: leading dot notation uses the expected type of the identifier to resolve it to a name, while field notation uses the inferred type of the term immediately prior to the dot.
+{tech}[Generalized field notation] is related: this {deftech}_leading dot notation_ uses the expected type of the identifier to resolve it to a name, while field notation uses the inferred type of the term immediately prior to the dot.
 
 Identifiers with a leading `.` are to be looked up in the {deftech}_expected type's namespace_.
 If the type expected for a term is a constant applied to zero or more arguments, then its namespace is the constant's name.
